semantics/alt_semantics/proofs/bigSmallEquivScript.sml
@@ -2271,7 +2271,7 @@ Proof
     Cases_on ‘store_assign n (Thunk Evaluated v) s.refs’ >> gvs[]
     )
   >- (
-    Cases_on ‘do_log l v e’ >> gvs[] >> Cases_on ‘x’ >> gvs[] >>
+    Cases_on ‘do_log a v e’ >> gvs[] >> Cases_on ‘x’ >> gvs[] >>
     metis_tac[big_clocked_total]
     )
   >- (Cases_on ‘do_if v e e0’ >> gvs[] >> metis_tac[big_clocked_total])
