semantics/alt_semantics/smallStepScript.sml
@@ -22,7 +22,7 @@ Datatype:
   | Chandle unit ((pat # exp) list)
   | Capp op (v list) unit (exp list)
   | Cforce num
-  | Clog lop unit exp
+  | Clog arith unit exp
   | Cif unit exp exp
   (* The value is raised if none of the patterns match *)
   | Cmat_check unit ((pat # exp) list) v
@@ -471,5 +471,3 @@ Definition small_decl_diverges_def:
     ==>
   (? c.  decl_step_reln env b c)))
 End
-
-
